PAC: duplicate sorting file

PAC/PAC_Polynoms_Operations.thy
@@ -56,7 +56,7 @@ lemma nonzero_coeffsD:
 lemma sorted_poly_list_rel_ConsD:
   \<open>((ys, n) # p, a) \<in> sorted_poly_list_rel S \<Longrightarrow> (p, remove1_mset (mset ys, n) a) \<in> sorted_poly_list_rel S \<and>
     (mset ys, n) \<in># a \<and> (\<forall>x \<in> set p. S ys (fst x)) \<and> sorted_wrt (rel2p var_order_rel) ys \<and>
-    distinct ys \<and> n \<noteq> 0 \<and> nonzero_coeffs a\<close>
+    distinct ys \<and> ys \<notin> set (map fst p) \<and> n \<noteq> 0 \<and> nonzero_coeffs a\<close>
   unfolding sorted_poly_list_rel_wrt_def prod.case mem_Collect_eq
     list_rel_def
   apply (clarsimp)
@@ -81,10 +81,10 @@ lemma sorted_poly_list_rel_ConsD:
 lemma sorted_poly_list_rel_Cons_iff:
   \<open>((ys, n) # p, a) \<in> sorted_poly_list_rel S \<longleftrightarrow> (p, remove1_mset (mset ys, n) a) \<in> sorted_poly_list_rel S \<and>
     (mset ys, n) \<in># a \<and> (\<forall>x \<in> set p. S ys (fst x)) \<and> sorted_wrt (rel2p var_order_rel) ys \<and>
-    distinct ys \<and> n \<noteq> 0 \<and> nonzero_coeffs a\<close>
+    distinct ys \<and> ys \<notin> set (map fst p) \<and> n \<noteq> 0 \<and> nonzero_coeffs a\<close>
   apply (rule iffI)
   subgoal
-    by (auto dest: sorted_poly_list_rel_ConsD)
+    by (auto dest!: sorted_poly_list_rel_ConsD)
   subgoal
     unfolding sorted_poly_list_rel_wrt_def prod.case mem_Collect_eq
       list_rel_def
@@ -96,6 +96,53 @@ lemma sorted_poly_list_rel_Cons_iff:
         nonzero_coeffs_def
       dest!: multi_member_split)
     done
+
+
+
+lemma sorted_repeat_poly_list_rel_ConsD:
+  \<open>((ys, n) # p, a) \<in> sorted_repeat_poly_list_rel S \<Longrightarrow> (p, remove1_mset (mset ys, n) a) \<in> sorted_repeat_poly_list_rel S \<and>
+    (mset ys, n) \<in># a \<and> (\<forall>x \<in> set p. S ys (fst x)) \<and> sorted_wrt (rel2p var_order_rel) ys \<and>
+    distinct ys \<and> n \<noteq> 0 \<and> nonzero_coeffs a\<close>
+  unfolding sorted_repeat_poly_list_rel_wrt_def prod.case mem_Collect_eq
+    list_rel_def
+  apply (clarsimp)
+  apply (subst (asm) list.rel_sel)
+  apply (intro conjI)
+  apply (rule_tac b = \<open>tl y\<close> in relcompI)
+  apply (auto simp: sorted_repeat_poly_list_rel_wrt_def list_mset_rel_def br_def)
+  apply (case_tac \<open>lead_coeff y\<close>; case_tac y)
+  apply (auto simp: term_poly_list_rel_def)
+  apply (case_tac \<open>lead_coeff y\<close>; case_tac y)
+  apply (auto simp: term_poly_list_rel_def)
+  apply (case_tac \<open>lead_coeff y\<close>; case_tac y)
+  apply (auto simp: term_poly_list_rel_def)
+  apply (case_tac \<open>lead_coeff y\<close>; case_tac y)
+  apply (auto simp: term_poly_list_rel_def)
+  apply (case_tac \<open>lead_coeff y\<close>; case_tac y)
+  apply (auto simp: term_poly_list_rel_def)
+  apply (case_tac \<open>lead_coeff y\<close>; case_tac y)
+  apply (auto simp: term_poly_list_rel_def nonzero_coeffs_def)
+  done
+
+lemma sorted_repeat_poly_list_rel_Cons_iff:
+  \<open>((ys, n) # p, a) \<in> sorted_repeat_poly_list_rel S \<longleftrightarrow> (p, remove1_mset (mset ys, n) a) \<in> sorted_repeat_poly_list_rel S \<and>
+    (mset ys, n) \<in># a \<and> (\<forall>x \<in> set p. S ys (fst x)) \<and> sorted_wrt (rel2p var_order_rel) ys \<and>
+    distinct ys \<and> n \<noteq> 0 \<and> nonzero_coeffs a\<close>
+  apply (rule iffI)
+  subgoal
+    by (auto dest!: sorted_repeat_poly_list_rel_ConsD)
+  subgoal
+    unfolding sorted_repeat_poly_list_rel_wrt_def prod.case mem_Collect_eq
+      list_rel_def
+    apply (clarsimp)
+    apply (intro conjI)
+    apply (rule_tac b = \<open>(mset ys, n) # y\<close> in relcompI)
+    by (auto simp: sorted_repeat_poly_list_rel_wrt_def list_mset_rel_def br_def
+        term_poly_list_rel_def add_mset_eq_add_mset eq_commute[of _ \<open>mset _\<close>]
+        nonzero_coeffs_def
+      dest!: multi_member_split)
+    done
+
 
 lemma add_poly_p_add_mset_sum_0:
    \<open>n + m = 0 \<Longrightarrow>add_poly_p\<^sup>*\<^sup>* (A, Aa, {#}) ({#}, {#}, r) \<Longrightarrow>
@@ -161,8 +208,9 @@ lemma add_poly_p_add_mset_comb3:
   by auto
 
 lemma total_on_lexord:
-  \<open>Relation.total_on R UNIV \<Longrightarrow> Relation.total_on (lexord R) UNIV\<close>
-  by (auto simp: Relation.total_on_def)
+  \<open>Relation.total_on UNIV R \<Longrightarrow> Relation.total_on UNIV (lexord R)\<close>
+  apply (auto simp: Relation.total_on_def)
+  by (meson lexord_linear)
 
 lemma antisym_lexord:
   \<open>antisym R \<Longrightarrow> irrefl R \<Longrightarrow> antisym (lexord R)\<close>
@@ -224,7 +272,7 @@ lemma add_poly_l'_add_poly_p:
         done
      done
     subgoal
-      apply (cases \<open>(xs, ys) \<in> lexord (lexord less_than_char)\<close>)
+      apply (cases \<open>(xs, ys) \<in> term_order_rel\<close>)
       subgoal
         using p(3)[of \<open>(remove1_mset (mset xs, n) (fst pq'), (snd pq'))\<close>] p(5-)
         apply (auto dest!: multi_member_split simp: sorted_poly_list_rel_Cons_iff rel2p_def)
@@ -235,7 +283,8 @@ lemma add_poly_l'_add_poly_p:
         apply assumption
         apply (auto intro: lexord_trans add_poly_p_add_mset_comb simp: lexord_transI
           sorted_poly_list_rel_nonzeroD)
-        done
+        using total_on_lexord_less_than_char_linear by fastforce
+
       subgoal
         using p(4)[of \<open>(fst pq', remove1_mset (mset ys, m) (snd pq'))\<close>] p(5-)
         apply (auto dest!: multi_member_split simp: sorted_poly_list_rel_Cons_iff rel2p_def)
@@ -248,7 +297,7 @@ lemma add_poly_l'_add_poly_p:
         apply assumption
         apply (auto intro: lexord_trans add_poly_p_add_mset_comb3 simp: lexord_transI
           sorted_poly_list_rel_nonzeroD)
-        done
+        using total_on_lexord_less_than_char_linear by fastforce
       done
    done
   done
@@ -271,11 +320,11 @@ lemma add_poly_l_spec:
 
 definition sort_poly_spec :: \<open>llist_polynom \<Rightarrow> llist_polynom nres\<close> where
 \<open>sort_poly_spec p =
-  SPEC(\<lambda>p'. mset p = mset p' \<and> sorted_wrt (rel2p (lexord var_order_rel)) (map fst p'))\<close>
+  SPEC(\<lambda>p'. mset p = mset p' \<and> sorted_wrt (rel2p (Id \<union> lexord var_order_rel)) (map fst p'))\<close>
 
 lemma sort_poly_spec_id:
   assumes \<open>(p, p') \<in> unsorted_poly_rel\<close>
-  shows \<open>sort_poly_spec p \<le> \<Down> (sorted_poly_rel) (RETURN p')\<close>
+  shows \<open>sort_poly_spec p \<le> \<Down> (sorted_repeat_poly_rel) (RETURN p')\<close>
 proof -
   obtain y where
     py: \<open>(p, y) \<in> \<langle>term_poly_list_rel \<times>\<^sub>r int_rel\<rangle>list_rel\<close> and
@@ -288,7 +337,7 @@ proof -
     by (auto simp: list_rel_def list_all2_conv_all_nth)
   have H: \<open>(x, p')
         \<in> \<langle>term_poly_list_rel \<times>\<^sub>r int_rel\<rangle>list_rel O list_mset_rel\<close>
-     if px: \<open>mset p = mset x\<close> and \<open>sorted_wrt (rel2p (lexord var_order_rel)) (map fst x)\<close>
+     if px: \<open>mset p = mset x\<close> and \<open>sorted_wrt (rel2p (Id \<union> lexord var_order_rel)) (map fst x)\<close>
      for x :: \<open>llist_polynom\<close>
   proof -
     obtain f where
@@ -322,7 +371,7 @@ proof -
   qed
   show ?thesis
     using zero
-    unfolding sort_poly_spec_def poly_list_rel_def sorted_poly_list_rel_wrt_def
+    unfolding sort_poly_spec_def poly_list_rel_def sorted_repeat_poly_list_rel_wrt_def
     by refine_rcg (auto intro: H)
 qed
 
@@ -591,17 +640,17 @@ lemma nonzero_coeffs_diff:
 
 
 lemma merge_coeffs_is_normalize_poly_p:
-  \<open>(xs, ys) \<in> sorted_poly_rel \<Longrightarrow> \<exists>r. (merge_coeffs xs, r) \<in> sorted_poly_rel \<and> normalize_poly_p\<^sup>*\<^sup>* ys r\<close>
+  \<open>(xs, ys) \<in> sorted_repeat_poly_rel \<Longrightarrow> \<exists>r. (merge_coeffs xs, r) \<in> sorted_poly_rel \<and> normalize_poly_p\<^sup>*\<^sup>* ys r\<close>
   apply (induction xs arbitrary: ys rule: merge_coeffs.induct)
-  subgoal by auto
+  subgoal by (auto simp: sorted_repeat_poly_list_rel_wrt_def sorted_poly_list_rel_wrt_def)
   subgoal
-    by auto
+    by (auto simp: sorted_repeat_poly_list_rel_wrt_def sorted_poly_list_rel_wrt_def)
   subgoal premises p for xs n ys m p ysa
     apply (cases \<open>xs = ys\<close>, cases \<open>m+n \<noteq> 0\<close>)
     subgoal
       using p(1)[of \<open>add_mset (mset ys, m+n) ysa - {#(mset ys, m), (mset ys, n)#}\<close>] p(4-)
       apply (auto simp: sorted_poly_list_rel_Cons_iff ac_simps add_mset_commute
-        remove1_mset_add_mset_If nonzero_coeffs_diff)
+        remove1_mset_add_mset_If nonzero_coeffs_diff sorted_repeat_poly_list_rel_Cons_iff)
       apply (rule_tac x = \<open>r\<close> in exI)
       using normalize_poly_p.merge_dup_coeff[of \<open>ysa -  {#(mset ys, m), (mset ys, n)#}\<close> \<open>ysa -  {#(mset ys, m), (mset ys, n)#}\<close> \<open>mset ys\<close> m n]
       apply (auto intro: normalize_poly_p.intros add_mset_commute add_mset_commute converse_rtranclp_into_rtranclp dest!: multi_member_split
@@ -610,24 +659,26 @@ lemma merge_coeffs_is_normalize_poly_p:
    subgoal
       using p(2)[of \<open>ysa - {#(mset ys, m), (mset ys, n)#}\<close>] p(4-)
       apply (auto simp: sorted_poly_list_rel_Cons_iff ac_simps add_mset_commute
-        remove1_mset_add_mset_If nonzero_coeffs_diff)
+        remove1_mset_add_mset_If nonzero_coeffs_diff sorted_repeat_poly_list_rel_Cons_iff)
       apply (rule_tac x = \<open>r\<close> in exI)
       using normalize_poly_p.rem_0_coeff[of \<open>add_mset (mset ys, m +n) ysa -  {#(mset ys, m), (mset ys, n)#}\<close> \<open>add_mset (mset ys, m +n) ysa -  {#(mset ys, m), (mset ys, n)#}\<close> \<open>mset ys\<close>]
       using normalize_poly_p.merge_dup_coeff[of \<open>ysa -  {#(mset ys, m), (mset ys, n)#}\<close> \<open>ysa -  {#(mset ys, m), (mset ys, n)#}\<close> \<open>mset ys\<close> m n]
       apply (auto intro: normalize_poly_p.intros add_mset_commute add_mset_commute converse_rtranclp_into_rtranclp dest!: multi_member_split
         simp del: normalize_poly_p.rem_0_coeff)
-      by (metis (no_types, hide_lams) add_mset_diff_bothsides converse_rtranclp_into_rtranclp diff_union_swap2 diff_zero
-        normalize_poly_p.rem_0_coeff p(4) same sorted_poly_list_rel_Cons_iff)
+      by (metis (no_types) add_mset_diff_bothsides converse_rtranclp_into_rtranclp diff_union_swap2 diff_zero
+        normalize_poly_p.rem_0_coeff p(4) same sorted_repeat_poly_list_rel_ConsD)
    subgoal
       using p(3)[of \<open>add_mset (mset ys, m) ysa - {#(mset xs, n), (mset ys, m)#}\<close>] p(4-)
     apply (auto simp: sorted_poly_list_rel_Cons_iff ac_simps add_mset_commute
-      remove1_mset_add_mset_If)
+      remove1_mset_add_mset_If sorted_repeat_poly_list_rel_Cons_iff)
     apply (rule_tac x = \<open>add_mset (mset xs, n) r\<close> in exI)
     apply (auto dest!: in_set_merge_coeffsD)
     apply (auto intro: normalize_poly_p.intros rtranclp_normalize_poly_add_mset
-      simp: var_order_rel_def
+      simp: var_order_rel_def rel2p_def
       dest!: multi_member_split
       dest: sorted_poly_list_rel_nonzeroD)
+     using total_on_lexord_less_than_char_linear apply fastforce
+     using total_on_lexord_less_than_char_linear apply fastforce
     done
   done
 done
